

We can easily extend eq. (11) to multiple examples  $\{s_1, s_2 \dots s_b\}$  and write the gradient descent update (using learning rate  $\eta$ ) equations as:

$$\begin{aligned} \dot{f}_\theta(s_j) &= -\eta \sum_i \tilde{\alpha}_i(s_j) w_i \quad , \quad \dot{w}_i = -\eta \sum_j \tilde{\alpha}_i(s_j) f_\theta(s_j) \\ \implies \dot{f}_\theta &= -\eta A W^T \quad , \quad \dot{W} = -\eta f_\theta^T A \end{aligned} \quad (12)$$

where

$$A_{ij} = \begin{cases} \alpha_j(s_i) - 1 & \text{if } c_i = j \\ \alpha_j(s_i) & \text{else} \end{cases} \quad (i^{th} \text{ example, } s_i, \text{ belongs to the class } j)$$

#### B.4. A useful matrix algebra result

**Lemma B.1.** *Let  $W(t)$  be a time-varying matrix with singular value decomposition (SVD):  $W(t) = U(t)S(t)V(t)^T$ , where  $U(t)$  and  $V(t)$  are orthogonal matrices corresponding to the left and right singular vectors, respectively, and  $S(t) = \text{diag}(\sigma_1(t), \sigma_2(t), \dots, \sigma_k(t))$  contains the singular values along its diagonal. Let  $u_k(t)$  and  $v_k(t)$  denote the  $k^{th}$  column vectors of  $U(t)$  and  $V(t)$ , respectively. Then the time derivative of the  $k^{th}$  singular value,  $\sigma_k(t)$ , is given by:*

$$\dot{\sigma}_k(t) = u_k(t)^T \dot{W}(t) v_k(t)$$

*Proof.* For sake of brevity, we will drop the explicit time-dependence of each matrix from the notations. Let us write the singular vector decomposition (SVD) of matrix,  $W = USV^T$ . Using the product rule of differentiation:

$$\begin{aligned} \dot{W} &= \dot{U}SV^T + U\dot{S}V^T + US\dot{V}^T \\ \implies U^T \dot{W} V &= U^T \dot{U} S + \dot{S} + S \dot{V}^T V \\ \implies \dot{S} &= U^T \dot{W} V - U^T \dot{U} S - S \dot{V}^T V \\ \implies \dot{\sigma}_k &= u_k^T \dot{W} v_k - u_k^T \dot{u}_k \sigma_k - \sigma_k \dot{v}_k^T v_k \end{aligned} \quad (13)$$

where the last line is the expression for the  $k^{th}$  diagonal element of  $S$ . By definition of orthonormal vectors,  $u_k^T u_k = 1$ . So,  $u_k^T \dot{u}_k + u_k^T \dot{u}_k = 0$ . Since  $u_k^T u_k$  is a scalar,  $u_k^T \dot{u}_k = -\dot{u}_k^T u_k$ . Therefore,  $u_k^T \dot{u}_k = 0$ . Similarly,  $\dot{v}_k^T v_k = 0$ . Therefore,

$$\dot{\sigma}_k = u_k^T \dot{W} v_k$$

□

#### B.5. Formal versions of theoretical results and proofs

**Theorem B.2.** *Let  $f_\theta = U_1 S_1 V_1^T$  and  $W = U_2 S_2 V_2^T$  denote the respective singular value decompositions (SVDs) of non-degenerate matrices  $f_\theta$  and  $W$ , respectively. If the system is initialized such that  $f_\theta^T f_\theta = W W^T$ , then it holds that:*

$$V_1 = U_2 \quad , \quad S_1^2 = S_2^2$$

*Proof.* Let us start from the learning dynamics imposed by gradient-descent:

$$\dot{f}_\theta = -\eta AW^T, \quad \dot{W} = -\eta f_\theta^T A \quad (14)$$

Let us write  $f_\theta$  and  $W$  as their respective singular value decomposed form, i.e. say  $f_\theta = U_1 S_1 V_1^T$  and  $W = U_2 S_2 V_2^T$ . Consider the dynamics of  $f_\theta^T f_\theta$  and  $WW^T$ :

$$\begin{aligned} \frac{d}{dt}(f_\theta^T f_\theta) &= \dot{f}_\theta^T f_\theta + f_\theta^T \dot{f}_\theta = (-\eta AW^T)^T f_\theta + f_\theta^T (-\eta AW^T) \\ &= -\eta W A^T f_\theta - \eta f_\theta^T A W^T \end{aligned} \quad (15)$$

$$\begin{aligned} \frac{d}{dt}(WW^T) &= \dot{W}W^T + W\dot{W}^T = (-\eta f_\theta^T A)W^T + W(-\eta f_\theta^T A)^T \\ &= -\eta f_\theta^T A W^T - \eta W A^T f_\theta \end{aligned} \quad (16)$$

From eqs. (15) and (16), it is clear that  $\frac{d}{dt}(f_\theta^T f_\theta) = \frac{d}{dt}(WW^T)$ , i.e.  $f_\theta^T f_\theta = WW^T + C$ , for some constant  $C$ . If we assume the initialization to be such that  $C = 0$  and  $f_\theta$  and  $W$  are non-degenerate, we have:

$$f_\theta^T f_\theta = WW^T \implies V_1 S_1^2 V_1^T = U_2 S_2^2 U_2^T$$

By uniqueness of SVD (for positive semi-definite matrices):

$$\begin{aligned} V_1 &= U_2 \implies V_1^T U_2 = I \\ S_1^2 &= S_2^2 \end{aligned}$$

□

**Theorem B.3.** Let  $f_\theta, W$  be the matrices whose dynamics are governed by the gradient-descent equations as previously defined. Given the conditions from Theorem B.2, the magnitude of the time derivatives of the  $i^{th}$  singular values of  $f_\theta$  and  $W$  are proportional to their respective singular values:

$$\begin{aligned} \|\dot{\sigma}_{1i}\| &\propto \sigma_{1i} \\ \|\dot{\sigma}_{2i}\| &\propto \sigma_{2i} \end{aligned}$$

Furthermore, assuming uniform class prediction at initialization and that number of classes,  $|\mathcal{V}| \gg 1$ , the time derivatives are bounded by the dominant class size:

$$\|\dot{\sigma}_{1i}\|, \|\dot{\sigma}_{2i}\| \propto \mathcal{O}(\mathcal{N}(c^{(0)}))$$

where  $\mathcal{N}(c^{(0)})$  denotes the number of instances belonging to the dominant class  $c^{(0)}$ .

*Proof.* Let us start from the results of Theorem B.2:  $S_1^2 = S_2^2 \implies \sigma_{1i}^2 = \sigma_{2i}^2 \forall i$ . So,  $\sigma_{1i} = \pm \sigma_{2i}$ . Using this relation, we can simplify the expression of  $\sigma_{1i}$  dynamics. From Theorem B.1,

$$\begin{aligned} \dot{\sigma}_{1i} &= u_{1i}^T \dot{f}_\theta v_{1i} = -\eta u_{1i}^T A W^T v_{1i} \\ &= -\eta u_{1i}^T A (U_2 S_2 V_2^T)^T v_{1i} = -\eta u_{1i}^T A V_2 S_2 U_2^T v_{1i} \\ &= -\eta u_{1i}^T A V_2 S_2 V_1^T v_{1i} \quad [\text{Using Theorem B.2}] \\ &= -\eta \sum_j (u_{1i}^T A v_{2j}) \sigma_{2j} (v_{1j} v_{1i}) = -\eta \sum_j (u_{1i}^T A v_{2j}) \sigma_{2j} \delta_{i=j} \\ \implies \dot{\sigma}_{1i} &= -\eta (u_{1i}^T A v_{2i}) \sigma_{2i} \end{aligned} \quad (17)$$

Similarly, we can simplify the dynamics for  $\sigma_{2i}$ :

$$\dot{\sigma}_{2i} = -\eta(u_{1i}^T A v_{2i}) \sigma_{1i} \quad (18)$$

For sake of brevity, let us denote  $(u_{1i}^T A v_{2i}) = g_i$ . Using the relationship between  $\sigma_{1i}$  and  $\sigma_{2i}$ , we can simplify eqs. (17) and (18) as:

$$\dot{\sigma}_{1i} = -\eta g_i (\pm \sigma_{1i}) = \mp \eta g_i \sigma_{1i} \quad , \quad \dot{\sigma}_{2i} = -\eta g_i (\pm \sigma_{2i}) = \mp \eta g_i \sigma_{2i} \quad (19)$$

$$\boxed{\implies \|\dot{\sigma}_{1i}\| \propto \sigma_{1i} \quad , \quad \|\dot{\sigma}_{2i}\| \propto \sigma_{2i}} \quad (20)$$

Also, note that  $g_i = u_{1i}^T A v_{2i} = \sum_{j,k} u_{1ij} A_{jk} v_{2ik}$ , where  $A_{jk} = \{\alpha_k(s_j) - 1, \alpha_k(s_j)\}$ . Therefore,  $A_{jk} \in (-1, 1)$ .

At initialization, WLOG  $\alpha_k(s_j) \approx \frac{1}{|\mathcal{V}|} \forall j, k$ , i.e. uniform class prediction. Additionally, assuming  $|\mathcal{V}| \gg 1$ , we can estimate  $g_i$  as the following:

$$\begin{aligned} g_i &= \sum_{j,k} u_{1ij} A_{jk} v_{2ik} = \sum_k \left( \sum_{j \in \{c_j=k\}} u_{1ij} (\alpha_k(s_j) - 1) v_{2ik} + \sum_{j \in \{c_j \neq k\}} u_{1ij} \alpha_k(s_j) v_{2ik} \right) \\ \implies g_i &\approx \sum_k \left( \left( \frac{1}{|\mathcal{V}|} - 1 \right) \sum_{j \in \{c_j=k\}} u_{1ij} v_{2ik} + \frac{1}{|\mathcal{V}|} \sum_{j \in \{c_j \neq k\}} u_{1ij} v_{2ik} \right) \\ &\approx - \left( \sum_k v_{2ik} \right) \left( \sum_{j \in \{c_j=k\}} u_{1ij} \right) = \mathcal{O}(\mathcal{N}(c^0)) \end{aligned} \quad (21)$$

where  $c^{(0)}$  denotes the dominant class, i.e. the class with most number of instances. Combining eq. (21) with eq. (19), we get the desired result:

$$\boxed{\|\dot{\sigma}_{1i}\|, \|\dot{\sigma}_{2i}\| \propto \mathcal{O}(\mathcal{N}(c^0))} \quad (22)$$

□